<!-- https://chatgpt.com/c/694e3cf0-66ac-8322-a177-0479105334cd -->

# 1

when solving for the range of a while there exists x, f a, x = 0. what are the methods.

---

When you’re asked to find **the range of a parameter (a)** such that **there exists (x)** with

$$
f(a,x)=0,
$$


you are solving an **existence problem**. There are several standard methods, and which one you use depends on the form of (f).

Below are the **main methods**, from most common to more advanced.

---

### 1. Treat it as an equation in (x) (most common)

Fix (a) and view

$$
f(a,x)=0
$$


as an equation in (x).

#### Steps

1. Rearrange into a standard form (polynomial, quadratic, etc.).
2. Ask: *for which values of (a) does this equation have at least one real solution?*
3. Use conditions like:

   * **Discriminant** ($\Delta \ge 0$) for quadratics
   * Factorability
   * Degree-based arguments

#### Example


$$
x^2 + ax + 1 = 0
$$


Exists real (x) ⇔

$$
\Delta = a^2 - 4 \ge 0 \Rightarrow |a| \ge 2
$$


---

### 2. Treat it as a function of (x) and use range/graphs

Rewrite:

$$
f(a,x)=0 \quad \Rightarrow \quad a = g(x)
$$


Then:

* The set of all possible (a) is the **range of (g(x))**.

#### Example


$$
ax + x^2 - 1 = 0 \Rightarrow a = \frac{1-x^2}{x}
$$


Find the range of

$$
g(x)=\frac{1-x^2}{x}
$$


(using calculus or algebra), and that range is the answer.

---

### 3. Use inequalities and extrema (calculus method)

If

$$
f(a,x)=0 \Rightarrow a = g(x)
$$


and (g(x)) has a **minimum or maximum**, then:

* (a) must lie between those extreme values.

#### Steps

1. Differentiate (g(x))
2. Find critical points
3. Compute min/max
4. State the range of (a)

This is very common in exam problems.

---

### 4. Complete the square (especially for quadratics in (x))

If the equation can be written as:

$$
(x - h)^2 = k(a)
$$


Then:

$$
k(a) \ge 0
$$


gives the condition on (a).

#### Example


$$
x^2 - 2ax + a + 1 = 0
$$



$$
(x-a)^2 = a^2 - a - 1
$$


Existence ⇔

$$
a^2 - a - 1 \ge 0
$$


---

### 5. Graphical interpretation

Interpret:

* (y=f(a,x))
* Solve (f(a,x)=0) ⇔ the graph intersects the (x)-axis

Then:

* Find for which (a) the graph **touches or crosses** the axis.

This helps especially with:

* Absolute values
* Piecewise functions
* Trigonometric equations

---

### 6. Special methods (advanced cases)

#### Trigonometric equations

Use bounds:

$$
-1 \le \sin x, \cos x \le 1
$$


#### Exponential / logarithmic equations

Use:

* Positivity constraints
* Monotonicity

#### Inequality-based existence

Sometimes you prove:

$$
\min_x f(a,x) \le 0 \le \max_x f(a,x)
$$


---

### Summary Table

| Situation              | Method                   |
| ---------------------- | ------------------------ |
| Polynomial in (x)      | Discriminant / factoring |
| Rearranged to (a=g(x)) | Range of function        |
| Quadratic form         | Complete the square      |
| Complicated (f)        | Calculus (min/max)       |
| Absolute/trig          | Bounds                   |
| Geometric              | Graph intersection       |

---

If you want, you can **share a specific function (f(a,x))** and I’ll show exactly which method works best and how to apply it step by step.

# 2

x(-x2+a)=-2x3/(x-1) when the right is positive

---

Nice — let’s solve it.

You gave the equation (I interpret `-x2` as $-x^2$ and `-2x3/(x-1)` as $-\dfrac{2x^3}{x-1}$)

$$
x(-x^2 + a);=; -\frac{2x^3}{,x-1,},
$$


and asked for the values of (a) for which this holds **when the right-hand side is positive**.

**Step 1 — solve for (a).**
Assuming $x\neq 1$ (denominator), rearrange:

$$
-x^3 + ax = -\frac{2x^3}{x-1}\quad\Rightarrow\quad a=\frac{x^2(x-3)}{x-1}.
$$


**Step 2 — impose the "right is positive" condition.**
Right-hand side positive means

$$
-\frac{2x^3}{x-1}>0 \quad\Longleftrightarrow\quad \frac{x^3}{x-1}<0.
$$


This inequality holds exactly for (0<x<1). (At (x=0) the RHS is (0), and (x=1) is not allowed.)

**Step 3 — find the range of (a) as (x) runs over ((0,1)).**
Consider (a(x)=\dfrac{x^2(x-3)}{x-1}) on ((0,1)). Compute derivative:

$$
a'(x)=\frac{2x(x^2-3x+3)}{(x-1)^2}>0\quad\text{for }0<x<1,
$$


so (a(x)) is strictly increasing on ((0,1)). Limits:

$$
\lim_{x\to0^+}a(x)=0,\qquad \lim_{x\to1^-}a(x)=+\infty.
$$


Thus the image of ((0,1)) under (a(x)) is ($0,\infty$).

**Conclusion.**
When the right-hand side is positive (i.e. for (x\in(0,1))), the possible values of (a) are exactly

$$
\boxed{a>0.}
$$


(For each (a>0) there is a unique (x\in(0,1)) solving the equation; (x=0) yields (a=0) but then RHS = 0, not positive.)

# 3

other methods

---

Great — here are several **different** ways (besides the derivative / direct monotonicity calculation you already saw) to handle the equation

$$
x(-x^2+a)=-\frac{2x^3}{x-1},
$$


under the condition that the right-hand side is positive (so (x\in(0,1))). I’ll give each method with a short, self-contained argument that leads to the same conclusion (a>0).

---

## 1 — **Algebraic rearrangement + limits / sign check (no calculus)**

Solve for (a) (for $x\ne1$, $x\ne0$ we can divide by (x)):

$$
a=\frac{x^2(x-3)}{x-1}.
$$


For (x\in(0,1)) the numerator (x^2(x-3)<0) and denominator (x-1<0), so (a>0).
Compute endpoint limits:

$$
\lim_{x\to0^+}a=;0,\qquad \lim_{x\to1^-}a=+\infty.
$$


Since (a(x)) is continuous on ((0,1)), its image contains every value between the limits, so the set of attainable (a) is ($0,\infty$).
(Concludes: (a>0).)

---

## 2 — **Intermediate Value Theorem (IVT) on a cleared-polynomial — constructive existence proof**

Clear denominators and factor out (x):

$$
x\bigl[(-x^2+a)(x-1)+2x^2\bigr]=0.
$$


For $x\ne0$ define

$$
F(x)=(-x^2+a)(x-1)+2x^2.
$$


Fix any (a>0). Evaluate endpoints of the open interval ((0,1)):

$$
\lim_{x\to0^+}F(x) = -a <0,\qquad \lim_{x\to1^-}F(x)=2>0.
$$


(F) is continuous on ((0,1)), so by IVT there is at least one root (x\in(0,1)). Thus for every (a>0) a solution with RHS positive exists; conversely (a) must be positive by sign argument in method 1.

---

## 3 — **Change of variable to remove the tricky denominator**

Use $x=\dfrac{y}{1+y}$ (maps (y\in$0,\infty$\leftrightarrow x\in(0,1))). Substitute into the expression for (a):

$$
a=\frac{x^2(x-3)}{x-1} \quad\Longrightarrow\quad
a=\frac{y^2(2y+3)}{(y+1)^2},\qquad y>0.
$$


This form is manifestly (>0) for all (y>0). Also $\lim_{y\to0^+}a=0$ and $\lim_{y\to\infty}a=\infty$, so the image is ($0,\infty$). This substitution often simplifies monotonicity/positivity checks.

(If you like, you can differentiate the (y)-form to show it’s strictly increasing — but that isn’t necessary once you see the limits and positivity.)

---

## 4 — **Graphical / comparison method**

Rewrite the original equation as

$$
x(-x^2+a) \quad\text{vs.}\quad -\frac{2x^3}{x-1}.
$$


For (x\in(0,1)) the right-hand side is positive and blows up as $x\to1^{-}$, while the left-hand side is continuous in (x) and equals $-a x^0$ near (0). By plotting (or comparing endpoint behaviour) you see that by varying (x\in(0,1)) the left expression spans from (0) up to arbitrarily large positive values (so the matching (a) spans ($0,\infty$)). This is the intuitive picture behind the IVT argument.

---

## 5 — **Algebraic long-division form — a useful identity**

Do polynomial division on $ $\dfrac{x^3-3x^2}{x-1}$$
to get
$$
a=\frac{x^3-3x^2}{x-1} = x^2-2x-2-\frac{2}{x-1}.
$$


This form can sometimes make asymptotics and sign easier to inspect (again gives the same behaviour as $x\to0^+$ and $x\to1^-$).

---

### Short summary / takeaways

* All methods show the same result: **the equation has a solution with the RHS positive iff (a>0)**; the possible values of (a) are ($0,\infty$).
* If you want a **calculus-free** existence proof use Method 2 (IVT after clearing denominators).
* If you want a **clean algebraic simplification**, use Method 3 (substitution (x=y/(1+y))) — it gives a manifestly positive rational in (y).

Would you like a quick plot or a numeric example showing (x) for several (a>0)? I can produce one and show the corresponding roots.

# 4

figure out it's increasing without derivative

---

Good question — this is a classic exam-style skill.
We’ll show the function is **increasing on ( (0,1) )** **without using derivatives**.

We already reduced the problem to

$$
a(x)=\frac{x^2(x-3)}{x-1},\qquad 0<x<1.
$$


---

### Method 1: Compare values directly (difference method)

Take two numbers

$$
0<x_1<x_2<1
$$


and compare (a$x_2$) and (a$x_1$).

Consider the difference:

$$
a(x_2)-a(x_1)
=\frac{x_2^2(x_2-3)}{x_2-1}-\frac{x_1^2(x_1-3)}{x_1-1}.
$$


Put over a common denominator:

$$
=\frac{(x_2-x_1),\bigl(2x_1x_2-x_1^2-x_2^2+3x_1+3x_2\bigr)}{(x_2-1)(x_1-1)}.
$$


Now check **signs** on ( (0,1) ):

* $x_2-x_1>0$
* ($x_2-1$$
x_1-1$>0) (product of two negatives)
* The bracket simplifies to
  [
  $x_1+x_2
$$3-x_1-x_2$ > 0
  \quad\text{since } x_1+x_2<2
  ]

So the whole fraction is **positive**, hence

$$
a(x_2)>a(x_1).
$$


✅ Therefore (a(x)) is **strictly increasing on ((0,1))**.

---

### Method 2: Rewrite as a sum of increasing functions

Do algebraic division:

$$
a(x)=x^2-2x-2-\frac{2}{x-1}.
$$


Now analyze each term on (0<x<1):

* $x^2$ → increasing
* (-2x) → decreasing
* constant (-2) → neutral
* $-\dfrac{2}{x-1}$ → **increasing** on ((0,1)) because (x-1<0) and the reciprocal becomes less negative as (x) increases

The strong increase from $-\frac{2}{x-1}$ dominates the linear decrease.
You can confirm by comparing values:

$$
x_2>x_1 \Rightarrow -\frac{2}{x_2-1}>-\frac{2}{x_1-1}.
$$


Adding preserves inequality, so the whole function increases.

---

### Method 3: Ratio monotonicity (smart factorization)

Rewrite:

$$
a(x)=x^2\cdot\frac{3-x}{1-x}.
$$


On (0<x<1):

* $x^2$ increases
* $\dfrac{3-x}{1-x}$ increases (numerator decreases slowly, denominator decreases faster)

Product of two positive increasing functions ⇒ increasing.

---

### Method 4: Endpoint squeezing + injectivity argument

* (a(x)) is continuous on ((0,1))
* (\displaystyle \lim_{x\to0^+}a(x)=0)
* (\displaystyle \lim_{x\to1^-}a(x)=+\infty)
* From the algebraic form, no two different (x) in ((0,1)) can give the same (a)

So the function must be strictly increasing (otherwise it would repeat values).

---

### Final takeaway

To prove monotonicity **without derivatives**, use:

1. **Difference sign method** (most rigorous)
2. **Rewrite as sum/product of monotone functions**
3. **Smart factorization**
4. **Continuity + injectivity**

If you want, I can show how this kind of argument is typically **phrased in exam marking schemes** so you can reproduce it cleanly under time pressure.

# 5

find out the value range without lim

---

Good — let’s do it **cleanly, rigorously, and with *no limits* at all**.

We work with

$$
a(x)=\frac{x^2(x-3)}{x-1},\qquad 0<x<1,
$$


and we already know (proved without derivatives) that **(a(x)) is strictly increasing on ((0,1))**.

---

### Step 1: Determine the **lower bound** (no limit)

Rewrite:

$$
a=\frac{x^2(x-3)}{x-1}.
$$


For (0<x<1):

* $x^2>0$
* (x-3<0)
* (x-1<0)

So numerator and denominator are both negative ⇒

$$
a>0.
$$


Now check whether (a=0) is possible:


$$
\frac{x^2(x-3)}{x-1}=0 \quad\Rightarrow\quad x^2(x-3)=0.
$$


This gives (x=0) or (x=3), **neither lies in ((0,1))**.

So:

$$
\boxed{a>0} \quad\text{and } 0 \text{ is NOT attained}.
$$


---

### Step 2: Show there is **no upper bound** (no limit)

We prove: for **any** (M>0), there exists (x\in(0,1)) such that (a>M).

Start from

$$
a=\frac{x^2(x-3)}{x-1}.
$$


Since (0<x<1), we have:

$$
x^2> \tfrac12 \quad \text{for all } x>\tfrac{1}{\sqrt2}.
$$


Also, for (x) sufficiently close to (1),

$$
\frac{1}{1-x} > \frac{M}{2}.
$$


Now rewrite:

$$
a = x^2\cdot\frac{3-x}{1-x}.
$$


For (x\in$\tfrac12,1$),

$$
x^2>\tfrac14,\qquad 3-x>2.
$$


So

$$
a > \tfrac14\cdot 2 \cdot \frac{1}{1-x} = \frac{1}{2(1-x)}.
$$


Choose (x) such that

$$
\frac{1}{2(1-x)}>M,
$$


which is always possible inside ((0,1)).

Hence, for any (M>0),

$$
\exists x\in(0,1):\ a>M.
$$


So **no finite upper bound exists**.

---

### Step 3: Use monotonicity to get the exact range

We now combine three facts:

1. (a(x)) is **strictly increasing** on ((0,1))
2. (a(x)>0) for all (x\in(0,1))
3. (a(x)) is **unbounded above**

A strictly increasing function on an interval that is always positive and unbounded above must have range:

$$
\boxed{(0,\infty)}.
$$


---

### ✅ Final Answer (no derivatives, no limits)


$$
\boxed{\text{Value range of } a \text{ is } (0,\infty).}
$$


---

If you want, I can also:

* show how this is written in **competition / Olympiad style**, or
* give a **one-paragraph exam-ready proof** you can memorize.

